feat: add missing theorems and simprocs to eliminate floats in a single pass (#11)
Co-authored-by: Abdalrhman Mohamed <abdal@barrett2.stanford.edu>

Fp/Theorems/ExtraTheorems.lean
@@ -1,12 +1,9 @@
 import Fp
 
-set_option maxHeartbeats 2000000
-
 -- Expansion
 
 theorem expand_preserves_value (a : EFixedPoint 34 16) (m : RoundingMode)
   : round 5 2 m (a.expand 38 18 (by omega) (by omega)) = round 5 2 m a := by
-  bv_float_normalize
   bv_decide
 
 theorem expand_self_is_id (a : EFixedPoint w e)
@@ -14,22 +11,18 @@ theorem expand_self_is_id (a : EFixedPoint w e)
   apply EFixedPoint.inj
   cases h : a.state <;> simp_all
 
-
 -- Comparison
 
 theorem e_lt_of_lt (a b : PackedFloat 5 2)
   : lt a b ↔ e_lt a.toEFixed b.toEFixed := by
-  bv_float_normalize
   bv_decide
 
 theorem le_of_e_le (m : RoundingMode) (a b : EFixedPoint 35 16)
   : e_le a b → le (round 5 2 m a) (round 5 2 m b) := by
-  bv_float_normalize
   bv_decide
 
 theorem e_le_of_le (a b : PackedFloat 5 2)
   : le a b ↔ e_le a.toEFixed b.toEFixed := by
-  bv_float_normalize
   bv_decide
 
 -- Rounding
@@ -40,7 +33,6 @@ floating point number.
 -/
 theorem toEFixed_isExactFloat (a : PackedFloat 5 2)
   : isExactFloat 5 2 a.toEFixed := by
-  bv_float_normalize
   bv_decide
 
 /--
@@ -49,20 +41,34 @@ floating point and back should not change the denotation.
 -/
 theorem isExactFloat_iff_round_toEFixed (a : EFixedPoint 34 16) (m : RoundingMode)
   : isExactFloat 5 2 a ↔ a.equal_denotation (round 5 2 m a).toEFixed := by
-  bv_float_normalize
+  -- Note: two issues occur if we remove the enum bound lemma below:
+  -- 1. `a.state` is assigned an arbitrary value outside of its bound
+  -- 2. `m` is assigned an arbitrary value outside of its bound
+  -- `bv_decide` currently cannot handle these cases for goals that require unfolding.
+  -- However, it can support them. The first issue doesn't matter much as we don't
+  -- plan to support `EFixedPoint` anyways. The second case,
+  -- however, is more important as we do want to support arbitrary
+  -- rounding modes. We're lucky here as the proof goes through anyway.
+  have : a.state.enumToBitVec < 0b11#2 := by cases a.state <;> decide
   bv_decide
+
+@[bv_normalize]
+def escapeEnumPass (m : RoundingMode) : Prop := m.enumToBitVec < 0b101#3
+
+theorem RoundingMode_enum_bound (m : RoundingMode)
+  : escapeEnumPass m := by
+  cases m <;> unfold escapeEnumPass <;> decide
+  -- bv_decide -- error: wrong counter-example
 
 /-- Fixed -> Float rounding is left inverse to Float -> Fixed conversion -/
 theorem round_leftinv_toEFixed (x : PackedFloat 5 2) (mode : RoundingMode):
   (round _ _ mode x.toEFixed).equal_denotation x := by
-  bv_float_normalize
   bv_decide
 
 -- Addition
 
 theorem f_add_comm (m : RoundingMode) (a b : FixedPoint 34 16)
   : (f_add m a b) = (f_add m b a) := by
-  bv_float_normalize
   bv_decide
 
 theorem e_add_comm (m : RoundingMode) (a b : EFixedPoint 34 16)
@@ -77,20 +83,17 @@ theorem add_comm (m : RoundingMode) (a b : PackedFloat 5 2)
 
 theorem add_neg_self_isZero_or_isNaN (a : PackedFloat 5 2) (m : RoundingMode)
   : (add a (neg a) m).isZero ∨ (add a (neg a) m).isNaN := by
-  bv_float_normalize
   bv_decide
 
 theorem add_zero_is_id (a : PackedFloat 5 2) (m : RoundingMode)
   (ha : ¬a.isNaN ∧ ¬a.isZero)
   : (add a (PackedFloat.getZero _ _) m) = a := by
-  bv_float_normalize
   bv_decide
 
 
 theorem e_add_monotone (m : RoundingMode) (a b c : EFixedPoint 34 16)
   (hc : c.state = .Number)
   : e_le a b → e_le (e_add m a c) (e_add m b c) := by
-  bv_float_normalize
   bv_decide
 
 theorem add_monotone (a b c : PackedFloat 5 2) (m : RoundingMode) (hc : c.isNormOrSubnorm)
@@ -111,7 +114,6 @@ operands are within a factor of two of each other.
 theorem sterbenz (a b : PackedFloat 5 2)
   (h : le a (doubleRNE b) ∧ le b (doubleRNE a))
   : isExactFloat 5 2 (e_add .RTZ a.toEFixed ((neg b).toEFixed)) := by
-  bv_float_normalize
   bv_decide
 
 -- Negation
@@ -122,7 +124,9 @@ theorem f_neg_involutive (a : FixedPoint 16 8)
 
 theorem e_neg_involutive (a : EFixedPoint 16 8)
   : (e_neg (e_neg a)).equal_denotation a := by
-  bv_float_normalize
+  -- Similar issue to the one discussed above.
+  -- Don't care about enum bounds for EFixedPoint.
+  bv_normalize
   bv_decide
 
 /--
@@ -130,7 +134,6 @@ Negation will always map an exact float to an exact float.
 -/
 theorem neg_exact (a : PackedFloat 5 2)
   : isExactFloat 5 2 (e_neg a.toEFixed) := by
-  bv_float_normalize
   bv_decide
 
 /--
@@ -138,7 +141,6 @@ theorem neg_exact (a : PackedFloat 5 2)
 -/
 theorem negfixed_eq_neg (a : PackedFloat 5 2) (m : RoundingMode)
   : negfixed a m = neg a := by
-  bv_float_normalize
   bv_decide
 
 /--
@@ -146,19 +148,14 @@ Applying `neg` twice gives you the identity.
 -/
 theorem neg_involutive (a : PackedFloat e s) (h : ¬a.isNaN)
   : neg (neg a) = a := by
-  have h' : ¬(neg a).isNaN := by
-    unfold neg
-    simp only [h]
-    simp_all
-  unfold neg at h' ⊢
-  simp only [h', h]
+  unfold neg at ⊢
+  simp only [h]
   simp_all
 
 -- Subtraction
 
 theorem subfixed_eq_sub (a b : PackedFloat 5 2) (m : RoundingMode)
   : subfixed a b m = sub a b m := by
-  bv_float_normalize
   bv_decide
 
 -- Multiplication
@@ -168,27 +165,22 @@ theorem subfixed_eq_sub (a b : PackedFloat 5 2) (m : RoundingMode)
 -/
 theorem mulfixed_eq_mul (a b : PackedFloat 5 2) (m : RoundingMode)
   : (mul a b m) = (mulfixed a b m) := by
-  bv_float_normalize
   bv_decide (timeout := 60)
 
 theorem mul_comm (a b : PackedFloat 5 2) (m : RoundingMode)
   : (mul a b m) = (mul b a m) := by
-  bv_float_normalize
   bv_decide
 
 theorem mul_one_is_id (a : PackedFloat 5 2) (m : RoundingMode)
   : (mul a oneE5M2 m).equal_denotation a := by
-  bv_float_normalize
   bv_decide
 
 theorem add_eq_mul_two (a : PackedFloat 5 2) (m : RoundingMode)
   : add a a m = mul twoE5M2 a m := by
-  bv_float_normalize
   bv_decide
 
 theorem doubleRNE_eq_mul_two (a : PackedFloat 5 2)
   : doubleRNE a = mul twoE5M2 a .RNE := by
-  bv_float_normalize
   bv_decide
 
 -- Fixed-point multiplication
@@ -212,20 +204,17 @@ theorem mulfixed_comm (a b : PackedFloat 5 2) (m : RoundingMode)
 
 theorem div_one_is_id (a : PackedFloat 5 2)
   : (div a oneE5M2 .RTZ).equal_denotation a := by
-  bv_float_normalize
   bv_decide
 
 theorem div_self_is_one (a : PackedFloat 5 2)
   (h : ¬a.isNaN ∧ ¬a.isInfinite ∧ ¬a.isZero)
   : (div a a .RTZ) = oneE5M2 := by
-  bv_float_normalize
   bv_decide
 
 -- Other
 
 theorem diff_zero_implies_equal (a b : PackedFloat 5 2) (m : RoundingMode)
   : (add a (neg b) m).isZero → ((a.isZero ∧ b.isZero) ∨ a = b) := by
-  bv_float_normalize
   bv_decide
 
 -- Square root
@@ -239,7 +228,6 @@ theorem rem_le_abs_self (a b : PackedFloat 5 2)
   (h : a.isNormOrSubnorm)
   (hb : ¬b.isNaN ∧ ¬b.isZero)
   : le (remainder a b) (abs b) := by
-    bv_float_normalize
     bv_decide
 
 /--
@@ -252,5 +240,4 @@ has to be exact.
 theorem remainder_doubling_homogeneous (a b : PackedFloat 5 2)
   (h : ¬(doubleRNE a).isInfinite ∧ ¬(doubleRNE b).isInfinite)
   : doubleRNE (remainder a b) = remainder (doubleRNE a) (doubleRNE b) := by
-  bv_float_normalize
   bv_decide
