Fp/Division.lean
@@ -1,7 +1,7 @@
 import Fp.Basic
 import Fp.Rounding
 
-@[bv_float_normalize]
+@[bv_normalize]
 def div_impl (a b : PackedFloat e s) (mode : RoundingMode) : PackedFloat e s :=
   let sign := a.sign ^^ b.sign
   let sig_a := BitVec.ofBool (a.ex ≠ 0) ++ a.sig
@@ -46,7 +46,7 @@ def div_impl (a b : PackedFloat e s) (mode : RoundingMode) : PackedFloat e s :=
 Division of two floating-point numbers, rounded to a floating point number
 using the provided rounding mode.
 -/
-@[bv_float_normalize]
+@[bv_normalize]
 def div (a b : PackedFloat e s) (mode : RoundingMode) : PackedFloat e s :=
   if a.isNaN ∨ b.isNaN ∨ (a.isInfinite ∧ b.isInfinite) ∨ (a.isZero ∧ b.isZero) then
     PackedFloat.getNaN _ _
