Fp/Subtraction.lean
@@ -6,7 +6,7 @@ import Fp.Negation
 /--
 Subtraction of two extended fixed-point numbers.
 -/
-@[bv_float_normalize]
+@[bv_normalize]
 def e_sub (mode : RoundingMode) (a b : EFixedPoint w e) : EFixedPoint (w+1) e :=
   e_add mode a (e_neg b)
 
@@ -15,7 +15,7 @@ Subtraction of two floating-point numbers.
 
 Implemented entirely within EFixedPoint using `e_sub`.
 -/
-@[bv_float_normalize]
+@[bv_normalize]
 def subfixed (a b : PackedFloat e s) (mode : RoundingMode) : PackedFloat e s :=
   round _ _ mode (e_sub mode a.toEFixed b.toEFixed)
 
@@ -24,6 +24,6 @@ Subtraction of two floating-point numbers.
 
 Implemented as a negation followed by an addition.
 -/
-@[bv_float_normalize]
+@[bv_normalize]
 def sub (a b : PackedFloat e s) (mode : RoundingMode) : PackedFloat e s :=
   add a (neg b) mode
