Fp/Tactics/Simps.lean
@@ -1,9 +1,45 @@
 import Fp.Tactics.Attributes
 
-attribute [bv_float_normalize] BitVec.setWidth'_eq
-attribute [bv_float_normalize] Eq.mp
-attribute [bv_float_normalize] ne_eq
-attribute [bv_float_normalize] beq_iff_eq
-attribute [bv_float_normalize] bne_iff_ne
-attribute [bv_float_normalize] Bool.or_eq_true
-attribute [bv_float_normalize] Bool.and_eq_true
+-- TODO: look into why these theorems are needed!
+attribute [bv_normalize] BitVec.setWidth'_eq
+attribute [bv_normalize] Eq.mp
+
+theorem ite_eq_cond {α} {c} [Decidable c] {b : Bool} {t e : α} (h : c = b)
+  : (if c then t else e) = (bif b then t else e) := by
+  simp [h]
+
+theorem dite_eq_cond {α} {c} [Decidable c] {b : Bool} {t e : α} (h : c = b)
+  : (if _ : c then t else e) = (bif b then t else e) := by
+  simp [h]
+
+theorem decide_eq_bool {p} [Decidable p] {b : Bool} (h : p = b)
+  : decide p = b := by
+  simp [h]
+
+open Lean Meta Simp in
+simproc ↓ [bv_normalize] ite_eq_cond_proc (@ite _ _ _ _ _) := fun e => do
+  let mkApp5 (.const ``ite [u]) α c hc t e := e | return .continue
+  let r ← simp c
+  let some (_, b, .const ``true _)  := r.expr.eq? | return .continue
+  let h ← r.getProof
+  return .visit { expr := mkApp4 (.const ``cond [u]) α b t e
+                  proof? := some (mkApp7 (.const ``ite_eq_cond [u]) α c hc b t e h) }
+
+open Lean Meta Simp in
+simproc ↓ [bv_normalize] dite_eq_cond_proc (@dite _ _ _ _ _) := fun e => do
+  let mkApp5 (.const ``dite [u]) α c hc (.lam _ _ t _) (.lam _ _ e _) := e | return .continue
+  if t.hasLooseBVars || e.hasLooseBVars then return .continue
+  let r ← simp c
+  let some (_, b, .const ``true _)  := r.expr.eq? | return .continue
+  let h ← r.getProof
+  return .visit { expr := mkApp4 (.const ``cond [u]) α b t e
+                  proof? := some (mkApp7 (.const ``dite_eq_cond [u]) α c hc b t e h) }
+
+open Lean Meta Simp in
+simproc ↓ [bv_normalize] decide_eq_bool_proc (@decide _ _) := fun e => do
+  let_expr decide p hp := e | return .continue
+  let r ← simp p
+  let some (_, b, .const ``true _)  := r.expr.eq? | return .continue
+  let h ← r.getProof
+  return .visit { expr := b
+                  proof? := some (mkApp4 (.const ``decide_eq_bool []) p hp b h) }
